Linglib/Studies/Larson1988.lean
@@ -3,7 +3,7 @@ Copyright (c) 2026 Robert Hawkins. All rights reserved.
 Released under Apache 2.0 license as described in the file LICENSE.
 Authors: Robert Hawkins
 -/
-import Linglib.Syntax.Minimalist.SyntacticObject.Subterm
+import Linglib.Syntax.Minimalist.SyntacticObject.Term
 import Linglib.Syntax.Minimalist.SyntacticObject.Build
 import Linglib.Syntax.Minimalist.Linearization.Replay
 import Linglib.Semantics.ArgumentStructure.Linking
