Linglib/Syntax/Minimalist/Movement/Freezing.lean
@@ -4,7 +4,7 @@ Released under Apache 2.0 license as described in the file LICENSE.
 Authors: Robert Hawkins
 -/
 import Linglib.Syntax.Minimalist.SyntacticObject.Derivation
-import Linglib.Syntax.Minimalist.SyntacticObject.Subterm
+import Linglib.Syntax.Minimalist.SyntacticObject.Term
 
 /-!
 # Freezing
